TM/Code/MatchProd.v
@@ -30,7 +30,7 @@ Section Projection.
       end.
 
 
-  Local Lemma CopySymbols_pair_first' (inputX : list sigX) (inputY : list sigY) tltr tl' tr' rs' :
+  Lemma CopySymbols_pair_first' (inputX : list sigX) (inputY : list sigY) tltr tl' tr' rs' :
     tape_local (fst tltr) = map inr (map inl inputX ++ map inr inputY) ++ (inl STOP :: rs') ->
     (tl', tr') = CopySymbols_Fun stop_X id tltr ->
     tape_local (tl') = map inr (map inr inputY) ++ (inl STOP :: rs').
@@ -45,7 +45,7 @@ Section Projection.
       + now rewrite map_app, <- app_assoc in H.
   Qed.
 
-  Local Lemma CopySymbols_pair_first'' (inputX : list sigX) (inputY : list sigY) ls m rs tr tl' tr' rs' :
+  Lemma CopySymbols_pair_first'' (inputX : list sigX) (inputY : list sigY) ls m rs tr tl' tr' rs' :
     m :: rs = map inr (map inl inputX ++ map inr inputY) ++ inl STOP :: rs' ->
     (tl', tr') = CopySymbols_Fun stop_X id (midtape ls m rs, tr) ->
     tape_local tl' = map inr (map inr inputY) ++ inl STOP :: rs'.
@@ -53,7 +53,7 @@ Section Projection.
     intros H1 H2. apply (CopySymbols_pair_first' (tltr := (midtape ls m rs, tr)) ltac:(cbn; eapply H1) H2).
   Qed.
 
-  Local Lemma CopySymbols_pair_second' (inputX : list sigX) (inputY : list sigY) tltr tl' tr' rs' :
+  Lemma CopySymbols_pair_second' (inputX : list sigX) (inputY : list sigY) tltr tl' tr' rs' :
     tape_local (fst tltr) = map inr (map inl inputX ++ map inr inputY) ++ (inl STOP :: rs') ->
     (tl', tr') = CopySymbols_Fun stop_X id tltr ->
     left tr' = map inr (map inl (rev inputX)) ++ left (snd tltr).
@@ -69,7 +69,7 @@ Section Projection.
       + trivial.
   Qed.
   
-  Local Lemma CopySymbols_pair_second'' (inputX : list sigX) (inputY : list sigY) ls m rs tr tl' tr' rs' :
+  Lemma CopySymbols_pair_second'' (inputX : list sigX) (inputY : list sigY) ls m rs tr tl' tr' rs' :
     m :: rs = map inr (map inl inputX ++ map inr inputY) ++ inl STOP :: rs' ->
     (tl', tr') = CopySymbols_Fun stop_X id (midtape ls m rs, tr) ->
     left tr' = map inr (map inl (rev inputX)) ++ left tr.
@@ -97,7 +97,7 @@ Section Projection.
       ).
 
   
-  Local Lemma M1_WRealise : M1 ⊫ R1.
+  Lemma M1_WRealise : M1 ⊫ R1.
   Proof.
     subst M1 R1.
     eapply WRealise_monotone.
@@ -125,7 +125,8 @@ Section Projection.
       - pose proof (CopySymbols_pair_second'' H2 H) as ->. now rewrite !map_rev.
     }
   Qed.
-  
+
+
   Definition Proj : { M : mTM (sigX+sigY)^+ 2 & states M -> unit } :=
     Inject (WriteMove (Some (inl START), R) tt) [|Fin.FS Fin.F1|];;
     M1;;
@@ -199,10 +200,91 @@ Section Projection.
   Qed.
 
 
-  (* TODO Termination *)
+  (** * Constructor *)
 
-  (* TODO: Konstruktor *)
+  (* TODO *)
+
+
+  (** * Termination *)
+
+  Lemma CopySymbols_TermTime_pair (x : X) (y : Y) (t : tape _) :
+    t ≂ (x, y) ->
+    CopySymbols_TermTime stop_X t <= 8 + 8 * length (encode x).
+  Proof.
+    intros (r1&r2&HE1&HE2). cbn -[plus mult] in *.
+    rewrite !map_app, <- app_assoc in HE2.
+    destruct (encode y) eqn:E1; cbn in HE2.
+    - pose proof CopySymbols_TermTime_local (stop := stop_X) HE2 ltac:(eauto). now rewrite !map_length in H.
+    - pose proof CopySymbols_TermTime_local (stop := stop_X) HE2 ltac:(eauto). now rewrite !map_length in H.
+  Qed.
+
   
+  Lemma M1_Terminates :
+    projT1 M1 ↓ (fun tin k => 
+                   exists (xy : X * Y),
+                     tin [@Fin.F1] ≂ xy /\
+                     12 + 8 * length (encode (fst xy)) <= k).
+  Proof.
+    unfold M1. eapply TerminatesIn_monotone.
+    {
+      repeat TM_Correct.
+      - eapply CopySymbols_WRealise.
+      - eapply CopySymbols_terminates.
+    }
+    {
+      cbn -[plus mult]. intros tin k. intros ((x&y)&HEncXY&Ht).
+      eexists. exists 3. repeat split.
+      - hnf in Ht. rewrite <- Ht. rewrite Nat.add_comm.
+        replace 11 with (3+8) by omega. replace (S (3 + 8)) with (4 + 8) by omega.
+        rewrite <- Nat.add_assoc. apply Nat.add_le_mono_l. cbn [fst].
+        eapply CopySymbols_TermTime_pair. eauto.
+      - intros tout (). intros H. hnf.
+        exists 1, 1. repeat split.
+        + omega.
+        + omega.
+        + intros tout' (). intros (?&?). clear_trivial_eqs. omega.
+    }
+  Qed.
+
+
+  Lemma Proj_Terminats :
+    projT1 Proj ↓ (fun tin k =>
+                   exists (xy : X * Y),
+                     tin [@Fin.F1] ≂ xy /\
+                     24 + 12 * length (encode (fst xy)) <= k).
+  Proof.
+    unfold Proj. eapply TerminatesIn_monotone.
+    {
+      repeat TM_Correct.
+      - apply M1_WRealise.
+      - apply M1_Terminates.
+      - apply MoveToSymbol_L_WRealise.
+      - apply MoveToSymbol_L_terminates.
+    }
+    {
+      cbn -[plus mult]. intros tin k. intros ((x&y)&HEncXY&Ht). cbn -[plus mult].
+      exists 1, (22 + 12 * length (encode x)). repeat split.
+      - assumption.
+      - hnf. omega.
+      - intros tout () ((_&H1)&H2). hnf in H1, H2. simpl_not_in. unfold finType_CS in *. rewrite <- !H2.
+        exists (12 + 8 * length (encode x)), (9 + 4 * length (encode x)). repeat split.
+        + omega.
+        + exists (x,y). split; eauto.
+        + intros tout2 () H3. specialize (H3 (x,y) ltac:(eauto)) as (H3&H4).
+          hnf. exists 1, (7 + 4 * length (encode x)). repeat split.
+          * omega.
+          * omega.
+          * intros tout3 () (_&H5). exists (4 + 4 * length (encode x)), 1. repeat split.
+            -- omega.
+            -- destruct H3 as (r1&r2&He1&He2). cbn -[plus mult] in *.
+               rewrite H4, H1 in H5. simpl_tape in H5.
+               assert (tape_local_l tout3[@Fin.F1] = rev (map inr (map inl (encode x))) ++ inl START :: left tin[@Fin.FS Fin.F1])
+                 as L by (rewrite H5; now simpl_tape).
+               pose proof MoveToSymbols_TermTime_local_l (stop := stop_X) L ltac:(eauto) as L2.
+               now rewrite rev_length, !map_length in L2.
+            -- intros tout4 [ | ]; intros; omega.
+    }
+  Qed.
+
 
 End Projection.
-
